## p39 伴随矩阵的性质证明
### 2. $(kA)^*=k^{n-1}A^*$
$(kA)^*=k^{n-1}A^* = |kA|(kA)^{-1} = k^n*|A|*\frac{1}{k}A^{-1} = k^{n-1}|A|A^{-1}=k^{n-1}A^*$

### 3. $(AB)^*=B^*A^*$
$|AB|*(AB)^{-1}=|A||B|*B^{-1}*A^{-1} = B^*A^*$

### 4.  $|A^*|=|A|^{n-1}$ 
 $|AA^*|=||A|*E|=|A|*|A^*|=|A|^{n} \rightarrow |A^*|=|A|^{n-1}$


### 5. $(A^*)^T=(A^T)^*$
$(A^*)^T=(|A|A^{-1})^T=|A|(A^{-1})^T$
$(A^T)^*=|A^T|(A^T)^{-1}$
$\because (A^T)^{-1} = (A^{-1})^{T}$
$\therefore (A^*)^T=(A^T)^*$
 

### 6. $(A^*)^{-1}=(A^{-1})^*=\frac{A}{|A|}$
$(A^*)^{-1}=(|A|A^{-1})^{-1}=\frac{(A^{-1})^{-1}}{|A|}=\frac{A}{|A|}$
$(A^{-1})^*=|A^{-1}|(A^{-1})^{-1}=\frac{A}{|A|}$

### 7. $(A^*)^*=|A|^{n-2}A$
